examples/scalaEquivalenceBenchmarkExamples/noHelp/max2.dfy
@@ -1,0 +1,29 @@
+// MODEL
+
+datatype List<T> = Nil | Cons(head: T, tail: List<T>)
+
+function maxM(lst: List<int>): int
+  decreases(lst) {
+  match lst {
+    case Nil             => -999999999999 // represent very small number
+    case Cons(hd, Nil)   => hd
+    case Cons(hd, tl)    => if (hd > maxM(tl)) then hd else maxM(tl)
+  }
+}
+
+function norm(l: List<int>, f: int): int {
+  match l
+    case Nil => -1
+    case _   => f
+}
+
+// CANDIDATE 1
+
+function max1(l: List<int>): int
+  decreases(l) {
+  match l {
+    case Nil           => 42
+    case Cons(hd, Nil) => hd
+    case Cons(hd, tl)    => if (hd > max1(tl)) then hd else max1(tl)
+  }
+}
