examples/scalaEquivalenceBenchmarkExamples/noHelp/sorting.dfy
@@ -1,0 +1,32 @@
+
+// Example 1: Check whether a list is sorted
+
+// Creating a list data structure
+datatype List<T> = Nil | Cons(head: T, tail: List<T>)
+
+// Defining isSortedR
+// This is the reference solution
+// Requires a clause to prove termination
+function loop(p: int, l: List<int>): bool
+  decreases l
+{
+  match l
+  case Nil => true
+  case Cons(x, xs) => p <= x && loop(x, xs)
+}
+
+function isSortedR(l: List<int>): bool
+{
+  match l
+  case Nil => true
+  case Cons(x, xs) => loop(x, xs)
+}
+
+// Defining isSortedB
+function isSortedB(l: List<int>): bool
+{
+  match l
+  case Nil => true
+  case Cons(x, Nil) => isSortedB(Nil)
+  case Cons(x, Cons(y, ys)) => x <= y && isSortedB(Cons(y, ys))
+}
