src/test/output/max2.dfy
@@ -1,0 +1,37 @@
+datatype List<A> = Nil | Cons(head: A, tail: List<A>)
+
+function maxM(lst: List<int>): int
+decreases (lst)
+{match lst {
+case Nil => -999999999999
+case Cons(hd, Nil) => hd
+case Cons(hd, tl) => if (hd > maxM(tl)) then hd else maxM(tl)
+}
+}
+
+function max1(l: List<int>): int
+decreases (l)
+{match l {
+case Nil => 42
+case Cons(hd, Nil) => hd
+case Cons(hd, tl) => if (hd > max1(tl)) then hd else max1(tl)
+}
+}
+
+function norm(l: List<int>, f: int): int
+{match l {
+case Nil => -1
+case _ => f
+}
+}
+
+lemma maxM_max1_Equivalence(lst: List<int>)
+decreases (lst)
+ensures (norm(lst, maxM(lst)) == norm(lst, max1(lst)))
+{{match lst {
+case Nil =>
+case Cons(hd, Nil) =>
+case Cons(hd, tl) =>maxM_max1_Equivalence(tl);if (hd > maxM(tl)){}else {maxM_max1_Equivalence(tl);}
+}
+}}
+
