src/test/output/sorting.dfy
@@ -1,0 +1,33 @@
+datatype List<A> = Nil | Cons(head: A, tail: List<A>)
+
+function isSortedR(l: List<int>): bool
+{match l {
+case Nil => true
+case Cons(x, xs) => loop(x, xs)
+}
+}
+
+function isSortedB(l: List<int>): bool
+{match l {
+case Nil => true
+case Cons(x, Nil) => isSortedB(Nil)
+case Cons(x, Cons(y, ys)) => ((x <= y) && isSortedB(Cons(y, ys)))
+}
+}
+
+function loop(p: int, l: List<int>): bool
+decreases (l)
+{match l {
+case Nil => true
+case Cons(x, xs) => ((p <= x) && loop(x, xs))
+}
+}
+
+lemma isSortedR_isSortedB_Equivalence(l: List<int>)
+ensures (isSortedR(l) == isSortedB(l))
+{{match l {
+case Nil =>
+case Cons(x, xs) =>
+}
+}}
+
